templates/lockfree/skiplist_v1_traverse.v
@@ -38,44 +38,45 @@ Module SKIPLIST1_SPEC_TRAVERSE.
   Admitted.
 
   Parameter findNext_spec : ∀ (n: Node) (i: nat),
-     ⊢ (<<< ∀∀ mark next k, node n mark next k >>>
-           findNext #n #i @ ⊤
-       <<< ∃∃ (m: bool) (opt_n': option Node),
-              node n mark next k ∗ ⌜mark !!! i = m⌝ ∗ ⌜next !! i = opt_n'⌝,
+    ⊢ <<< ∀∀ h mark next k, node n h mark next k ∗ ⌜i < h⌝ >>>
+          findNext #n #i @⊤
+      <<< ∃∃ (m: bool) (opt_n': option Node),
+              node n h mark next k ∗ ⌜mark !!! i = m⌝ ∗ ⌜next !! i = opt_n'⌝,
               RET (match opt_n' with None => (#m, NONEV) 
-                                    | Some n' => (#m, SOMEV #n') end) >>>)%I.
+                                    | Some n' => (#m, SOMEV #n') end) >>>.
 
-  Parameter try_constraint_traverse_spec : ∀ (pred curr new_node: Node) (i: nat),
-     ⊢ (<<< ∀∀ mark next k, node pred mark next k >>>
-           try_constraint #pred #curr #new_node #i @ ⊤
-       <<< ∃∃ (success: bool) next',
-              node pred mark next' k
-            ∗ (match success with true => ⌜next !! i = Some curr 
+  Parameter changeNext_spec : ∀ (n m m': Node) (i: nat),
+    ⊢  <<< ∀∀ h mark next k, node n h mark next k ∗ ⌜i < h⌝ >>>
+            changeNext #n #m #m' #i @⊤
+      <<< ∃∃ (success: bool) next',
+              node n h mark next' k
+            ∗ (match success with true => ⌜next !! i = Some m 
                                             ∧ mark !!! i = false
-                                            ∧ next' = <[i := new_node]> next⌝
-                                | false => ⌜(next !! i ≠ Some curr ∨ 
+                                            ∧ next' = <[i := m']> next⌝
+                                | false => ⌜(next !! i ≠ Some m ∨ 
                                               mark !!! i = true)
                                             ∧ next' = next⌝ end),
               RET (match success with true => SOMEV #() 
-                                    | false => NONEV end)  >>>)%I.
+                                    | false => NONEV end)  >>>.
 
   Parameter compareKey_spec : ∀ (n: Node) (k': nat),
-     ⊢ (<<< ∀∀ mark next k, node n mark next k >>>
+    ⊢ <<< ∀∀ h mark next k, node n h mark next k >>>
            compareKey #n #k' @ ⊤
-       <<< ∃∃ (res: nat),
-              node n mark next k ∗ 
-              ⌜if decide (res = 0) then k < k'
-               else if decide (res = 1) then k = k'
-               else k > k'⌝,
-              RET #res >>>)%I.
-                                    
+     <<< ∃∃ (res: nat),
+            node n h mark next k 
+          ∗ ⌜if decide (res = 0) then k < k'
+             else if decide (res = 1) then k = k'
+             else k > k'⌝,
+         RET #res >>>.
 
   Definition traversal_inv s i k p c : Prop :=
     p ∈ FP s 
   ∧ c ∈ FP s 
   ∧ Key s p < k 
   ∧ Marki s p i = false 
-  ∧ Nexti s p i = Some c.
+  ∧ Nexti s p i = Some c
+  ∧ i < Height s p
+  ∧ i < Height s c.
 
   Lemma traverse_i_spec N γ_t γ_r γ_m γ_td1 γ_td2 γ_ght
   γ_sy t_id t0 k (i: nat) (p c: Node):
@@ -109,10 +110,12 @@ Module SKIPLIST1_SPEC_TRAVERSE.
     { (* interpolation *) admit. }
     rewrite (big_sepS_delete _ (FP s0) c); last by eauto.
     iDestruct "Nodes" as "(Node_c & Nodes_rest)".
-    iAaccIntro with "Node_c".
-    { iIntros "Node". iModIntro. iFrame "Hpost".
-      iNext; iExists M0, T0, s0.
-      iFrame "∗%#". 
+    iAssert ((node c (Height s0 c) (Mark s0 c) (Next s0 c) (Key s0 c)) 
+      ∗ ⌜i < Height s0 c⌝)%I with "[Node_c]" as "Hpre".
+    { admit. }
+    iAaccIntro with "Hpre".
+    { iIntros "(Node_c & _)". iModIntro. iFrame "Hpost".
+      iNext; iExists M0, T0, s0. iFrame "∗%#". 
       rewrite (big_sepS_delete _ (FP s0) c); last by eauto. 
       iFrame "Nodes_rest". iFrame. }
     iIntros (m c') "(Node_c & %Mark_c0 & %Next_c0)".
@@ -121,7 +124,7 @@ Module SKIPLIST1_SPEC_TRAVERSE.
       rewrite (big_sepS_delete _ (FP s0) c); last by eauto.
       iFrame "Nodes_rest". iFrame. }
     destruct c' as [cn |]; destruct m; wp_pures. 
-    - awp_apply try_constraint_traverse_spec; try done.
+    - awp_apply changeNext_spec; try done.
       iInv "HInv" as (M1 T1 s1) "(>Ds & >%Habs1 & >Hist & Help & >Templ)".
       { admit. }
       iDestruct "Templ" as "(SShot1 & Res & %PT1 & %Trans_M1)".
@@ -130,16 +133,19 @@ Module SKIPLIST1_SPEC_TRAVERSE.
       { (* interpolation *) admit. }
       rewrite (big_sepS_delete _ (FP s1) p); last by eauto.
       iDestruct "Nodes" as "(Node_p & Nodes_rest)".
-      iAaccIntro with "Node_p".
-      { iIntros "Node_p". iModIntro. iFrame "Hpost".
+      iAssert ((node p (Height s1 p) (Mark s1 p) (Next s1 p) (Key s1 p)) 
+        ∗ ⌜i < Height s1 p⌝)%I with "[Node_p]" as "Hpre".
+      { admit. }
+      iAaccIntro with "Hpre".
+      { iIntros "(Node_p&_)". iModIntro. iFrame "Hpost".
         iNext; iExists M1, T1, s1. iFrame "∗%#". 
         rewrite (big_sepS_delete _ (FP s1) p); last by eauto. iFrame. }
       iIntros (success next') "(Node_p & Hsuccess)".
       destruct success.
       + iDestruct "Hsuccess" as %[Next_p1 [Mark_p1 Def_next']].
         destruct (decide (i = 0)) as [-> | Hi0].
-        * iDestruct "SShot1" as %[FP1 [C1 [Mk1 [Nx1 [Ky1 [I1 
-            [Hs1 [Dom_Mk1 [Dom_Nx1 [Dom_Ky1 Dom_I1]]]]]]]]]].
+        * iDestruct "SShot1" as %[FP1 [C1 [Ht1 [Mk1 [Nx1 [Ky1 [I1 
+            [Hs1 [Dom_Ht1 [Dom_Mk1 [Dom_Nx1 [Dom_Ky1 Dom_I1]]]]]]]]]]]].
           set Nx1' := <[p := next']> Nx1.
           set Ip1 := I1 !!! p. set Ic1 := I1 !!! c. set out_pc := out Ip1 c.
           set Ip1' := int {| infR := inf_map Ip1; outR :=  <<[cn := out_pc]>> ∅ |}.
@@ -147,7 +153,7 @@ Module SKIPLIST1_SPEC_TRAVERSE.
             int {| infR := {[c := (inf Ic1 c - out_pc)%CCM]}; 
                   outR := <<[cn := (out Ic1 cn - out_pc)%CCM]>> ∅ |}.
           set I1' := <[c := Ic1']> (<[p := Ip1']> I1).
-          set s1' := (FP1, C1, Mk1, Nx1', Ky1, I1'): snapshot.
+          set s1' := (FP1, C1, Ht1, Mk1, Nx1', Ky1, I1'): snapshot.
           set M1' := <[T1 + 1 := s1']> M1.
           iAssert (⌜per_tick_inv s1⌝)%I as %PT_s1.
           { iDestruct "Hist" as (M')"(_&_&_&%&_)". iPureIntro.
@@ -164,11 +170,11 @@ Module SKIPLIST1_SPEC_TRAVERSE.
             by pose proof PT p c 0 Next_p1. }
           assert (Key s1 p < W) as Key_p1.
           { destruct PT_s1 as (_&_&PT&_). apply PT in FP_c1.
-            destruct FP_c1 as (_&_&_&_&H'&_). clear -H' Key_pc. lia. }
+            destruct FP_c1 as (_&_&_&_&_&H'&_). clear -H' Key_pc. lia. }
           assert (∀ x, x ∈ FP s1 → flow_constraints_I x (FI s1 x) 
                   (Mark s1 x !!! 0) (Next s1 x !! 0) (Key s1 x)) as Hflow.
           { destruct PT_s1 as (_&_&H'&_).
-            intros x Hx. apply H' in Hx. by destruct Hx as (_&_&_&_&_&?). }
+            intros x Hx. apply H' in Hx. by destruct Hx as (_&_&_&_&_&_&?). }
           assert (∀ x, I1 !!! x = FI s1 x) as I1_eq_s1.
           { intros x. rewrite Hs1; unfold FI. try done. }
           assert (flow_constraints_I p Ip1 false (Some c) (Key s1 p)) as Hp.
@@ -176,6 +182,8 @@ Module SKIPLIST1_SPEC_TRAVERSE.
           assert (flow_constraints_I c Ic1 true (Some cn) (Key s1 c)) as Hc.
           { apply Hflow in FP_c1. by rewrite -I1_eq_s1 Next_c1 Mark_c1 in FP_c1. }
           assert (insets Ip1 ≠ ∅) as Inset_p1_ne.
+          { admit. }
+          assert (insets Ic1 ≠ ∅) as Inset_c1_ne.
           { admit. }
           assert (out_pc ≠ 0%CCM) as Out_pc.
           { destruct Hp as (_&H'&_&(_&H'')&_). rewrite /outsets H' in H''. 
@@ -186,10 +194,6 @@ Module SKIPLIST1_SPEC_TRAVERSE.
             rewrite /outset in H''. rewrite -nzmap_elem_of_dom_total2 in H'.
             rewrite -I1_eq_s1 -H'' in H'. apply H'. 
             rewrite elem_of_gset_seq. clear -Key_p1; split; lia. done. }
-          (*
-          assert (inf Ic1 c = out_pc) as Inf_Ic1.
-          { admit. }
-          *)
           assert (out Ic1 cn = inf Ic1 c) as Out_Ic1.
           { admit. }
           assert (p ≠ c) as p_neq_c.
@@ -198,13 +202,17 @@ Module SKIPLIST1_SPEC_TRAVERSE.
           { admit. }
           assert (c ≠ cn) as c_neq_cn.
           { admit. }
-          assert (dom Ip1 = {[p]}) as Dom_Ip1.
-          { admit. }
-          assert (dom Ic1 = {[c]}) as Dom_Ic1.
-          { admit. }
+          assert (dom Ip1 = {[p]}) as Dom_Ip1 by apply Hp.
+          assert (dom Ic1 = {[c]}) as Dom_Ic1 by apply Hc.
           assert (dom Ip1' = {[p]}) as Dom_Ip1'.
-          { admit. }
+          { rewrite /dom /flowint_dom /Ip1' /=. apply Dom_Ip1. }
           assert (dom Ic1' = {[c]}) as Dom_Ic1'.
+          { by rewrite /dom /flowint_dom /Ip1' /= dom_singleton_L. }
+          assert (dom (out_map Ip1) = {[c]}) as Domout_Ip1.
+          { admit. }
+          assert (dom (out_map Ic1) = {[cn]}) as Domout_Ic1.
+          { admit. }
+          assert (dom (out_map Ip1') = {[cn]}) as Domout_Ip1'.
           { admit. }
           assert (✓ (Ip1 ⋅ Ic1)) as Vpc1.
           { admit. }
@@ -215,7 +223,8 @@ Module SKIPLIST1_SPEC_TRAVERSE.
             - rewrite /dom /flowint_dom in Dom_Ip1. rewrite Dom_Ip1.
               rewrite nzmap_dom_insert_nonzero. clear -p_neq_cn; set_solver.
               done.
-            - intros H'. admit.
+            - intros H'. rewrite /dom /flowint_dom H' in Dom_Ip1.
+              clear -Dom_Ip1; set_solver.
             - clear -c_neq_cn. rewrite dom_insert dom_empty.
               destruct (decide ((out Ic1 cn - out_pc)%CCM = 0%CCM)).
               rewrite nzmap_dom_insert_zero; try done. 
@@ -234,7 +243,7 @@ Module SKIPLIST1_SPEC_TRAVERSE.
               assert (out Ic1' p = 0%CCM) as ->. 
               { rewrite /out /Ic1' /out_map /= nzmap_lookup_total_insert_ne.
                 rewrite nzmap_lookup_empty. all: done. }
-              admit.
+              by rewrite ccm_left_id ccm_pinv_unit.
             - apply map_Forall_lookup. intros i m. 
               destruct (decide (i = c)) as [-> | Hic].
               + rewrite lookup_insert. intros [=<-].
@@ -244,7 +253,7 @@ Module SKIPLIST1_SPEC_TRAVERSE.
                 assert ((inf Ic1 c - out_pc)%CCM = inf Ic1' c) as ->.
                 { by rewrite /Ic1' {2}/inf /inf_map /= lookup_insert /=. }
                 rewrite /inf /Ic1' /inf_map /= lookup_insert /=.
-                admit.
+                by rewrite ccm_left_id ccm_pinv_unit.
               + rewrite lookup_insert_ne; try done. }
           assert (dom (Ip1 ⋅ Ic1) = {[p;c]}) as Dom_pc.
           { rewrite intComp_dom; try done. rewrite Dom_Ip1 Dom_Ic1; done. } 
@@ -262,7 +271,9 @@ Module SKIPLIST1_SPEC_TRAVERSE.
                 { rewrite /out /Ic1' /out_map /= nzmap_lookup_total_insert_ne.
                   rewrite nzmap_lookup_empty. all: done. }
                 assert (out Ic1 p = 0%CCM) as ->.
-                { admit. }
+                { rewrite /out -nzmap_elem_of_dom_total2.
+                  destruct Hc as (_&Hc&_). rewrite Hc; try done.
+                  clear -p_neq_cn; set_solver. }
                 done. rewrite Dom_Ip1; clear; set_solver.
                 rewrite Dom_Ip1'; clear; set_solver.
               + destruct (decide (n = c)) as [-> | Hnc]; last first.
@@ -278,8 +289,8 @@ Module SKIPLIST1_SPEC_TRAVERSE.
                 { rewrite /out /Ip1' /out_map /=.
                   rewrite nzmap_lookup_total_insert_ne; try done. }
                 rewrite {1}/inf /Ic1' /inf_map /= lookup_insert /= /out_pc.
-                admit. rewrite Dom_Ic1. clear; set_solver. rewrite Dom_Ic1'.
-                clear; set_solver.
+                by rewrite ccm_pinv_unit. rewrite Dom_Ic1. clear; set_solver. 
+                rewrite Dom_Ic1'. clear; set_solver.
             - intros n. destruct (decide (n ∈ ({[p;c]}: gset Node))) as [Hn | Hn].
               { rewrite !intValid_in_dom_not_out; try done.
                 by rewrite Dom_pc. by rewrite Dom_pc'. }
@@ -290,8 +301,16 @@ Module SKIPLIST1_SPEC_TRAVERSE.
                 assert (out Ic1' cn = (out Ic1 cn - out_pc)%CCM) as ->.
                 { by rewrite /Ic1' /out /= nzmap_lookup_total_insert. }
                 assert (out Ip1 cn = 0%CCM) as ->.
-                { admit. }
-                rewrite Out_Ic1 /out_pc. admit.
+                { rewrite /out -nzmap_elem_of_dom_total2.
+                  destruct Hp as (_&Hp&_). rewrite Hp; try done.
+                  clear -c_neq_cn; set_solver. }
+                rewrite Out_Ic1 /out_pc. rewrite ccm_left_id.
+                apply intComposable_valid in Vpc1. destruct Vpc1 as (_&_&_&_&H'). 
+                rewrite map_Forall_lookup in H'. pose proof H' c (inf Ic1 c) as H'.
+                rewrite {2}H'. done. rewrite /inf. assert (c ∈ dom Ic1) as H''.
+                rewrite Dom_Ic1; clear; set_solver. 
+                rewrite /dom /flowint_dom elem_of_dom in H''. 
+                destruct H'' as [m ->]. by simpl.
               + assert (out Ip1' n = 0%CCM) as ->. 
                 { rewrite /out /Ip1' /= nzmap_lookup_total_insert_ne; try done. }
                 assert (out Ic1' n = 0%CCM) as ->.
@@ -303,21 +322,60 @@ Module SKIPLIST1_SPEC_TRAVERSE.
                 done.
               + by rewrite Dom_pc.
               + by rewrite Dom_pc'. }
+          assert (insets Ip1' = insets Ip1) as Insets_Ip1'.
+          { rewrite /insets Dom_Ip1 Dom_Ip1' /inset /inf /=. done. }
+          assert (outsets Ip1' = outsets Ip1) as Outsets_Ip1'.
+          { destruct Hp as (_&Hp&_). rewrite /outsets Hp /Ip1 /=; try done.
+            assert (dom <<[cn := out_pc]>> ∅ = {[cn]}) as ->.
+            apply leibniz_equiv. rewrite nzmap_dom_insert_nonzero; try done.
+            rewrite /dom. clear; set_solver. apply leibniz_equiv.
+            rewrite !big_opS_singleton. rewrite /outset /Ip1' {1}/out /=.
+            rewrite nzmap_lookup_total_insert /out_pc /Ip1. done. }
           assert (flow_constraints_I p Ip1' false (Some cn) (Key s1 p)) as Hp'.
           { destruct Hp as (Hp1&Hp2&Hp3&Hp4&Hp5&Hp6&Hp7). 
             split; last split; last split; last split; last split; 
               last split; try done.
-            - intros _. rewrite /Ip1' /=. apply leibniz_equiv. 
-              rewrite nzmap_dom_insert_nonzero; try done.
-              rewrite /dom. clear; set_solver.
-            - admit.
-            - admit.
-            - admit. }
+            - rewrite Insets_Ip1' Outsets_Ip1'. done.
+            - rewrite Insets_Ip1' Outsets_Ip1'. done.
+            - intros n' k'. destruct (decide (n' = cn)) as [-> | Hn'cn].
+              + assert (out Ip1' cn = out_pc) as ->.
+                { by rewrite /out /Ip1' /= nzmap_lookup_total_insert. }
+                pose proof Hp7 c k' as H'. apply H'.
+              + assert (out Ip1' n' = 0%CCM) as ->.
+                { rewrite /out /Ip1' /= nzmap_lookup_total_insert_ne; try done. }
+                rewrite nzmap_lookup_empty. rewrite /ccmunit /= /nat_unit. lia. }
           set S := dom out_pc.
           assert (S ⊆ insets Ic1) as S_sub_c1.
           { admit. }
-          assert (insets Ic1' = insets Ic1 ∖ S) as Insets_Ic1'.
+          assert (∀ k', inf Ic1 c !!! k' ≤ 1) as HInf_Ic1.
           { admit. }
+          assert (∀ k', out_pc !!! k' ≤ 1) as Hout_pc.
+          { admit. }
+          assert (insets Ic1' = insets Ic1 ∖ S) as Insets_Ic1'.
+          { rewrite /insets Dom_Ic1' Dom_Ic1. apply leibniz_equiv. 
+            rewrite !big_opS_singleton. 
+            assert (inset _ Ic1' c = dom (inf Ic1 c - out_pc)%CCM) as ->.
+            { rewrite /inset {1}/inf /=  lookup_insert /=. done. }
+            rewrite /inset /S. rewrite set_equiv_subseteq.
+            split. intros k' Hk'. apply nzmap_elem_of_dom_total in Hk'.
+            rewrite lookup_total_lifting_inv in Hk'. rewrite elem_of_difference.
+            rewrite /ccmunit /= /nat_unit /ccmop_inv /ccm_opinv /= 
+              /nat_opinv in Hk'. 
+            assert (inf Ic1 c !!! k' = 1 ∧ out_pc !!! k' = 0) as [H' H''].
+            { pose proof HInf_Ic1 k' as H'. pose proof Hout_pc k' as H''.
+              set a := inf Ic1 c !!! k'. set b := out_pc !!! k'.
+              rewrite -/a in H'. rewrite -/b in H''. rewrite -/a -/b in Hk'.
+              clear -H' H'' Hk'; split; try lia. }
+            split. rewrite nzmap_elem_of_dom_total H' /ccmunit /= /nat_unit. 
+            clear; lia. rewrite nzmap_elem_of_dom_total2 H''. 
+            by rewrite /ccmunit /= /nat_unit.
+            intros k' Hk'. rewrite elem_of_difference in Hk'.
+            destruct Hk' as [Hk1' Hk2']. rewrite nzmap_elem_of_dom_total in Hk1'.
+            rewrite /ccmunit /= /nat_unit in Hk1'.
+            rewrite nzmap_elem_of_dom_total2 /ccmunit /= /nat_unit in Hk2'.
+            rewrite nzmap_elem_of_dom_total /ccmunit /= /nat_unit /ccmop_inv.
+            rewrite lookup_total_lifting_inv /ccmop_inv /ccm_opinv /= /nat_opinv.
+            rewrite Hk2'. clear -Hk1'; lia. }
           assert (outsets Ic1' = outsets Ic1 ∖ S) as Outsets_Ic1'.
           { admit. }
           assert (flow_constraints_I c Ic1' true (Some cn) (Key s1 c)) as Hc'.
@@ -328,19 +386,153 @@ Module SKIPLIST1_SPEC_TRAVERSE.
               rewrite nzmap_dom_insert_nonzero; try done.
               rewrite /dom. clear; set_solver. rewrite Out_Ic1.
               rewrite /insets Dom_Ic1' -leibniz_equiv_iff in H'. 
-              rewrite big_opS_singleton /inset /Ic1' {1}/inf /= lookup_insert /= in H'.
+              rewrite big_opS_singleton /inset /Ic1' {1}/inf /= 
+                lookup_insert /= in H'.
               intros H''. rewrite H'' in H'. apply H'.
               rewrite /ccmunit /=. clear; set_solver.
             - rewrite Insets_Ic1' Outsets_Ic1'. clear -Hc3 S_sub_c1; set_solver.
             - rewrite /keyset Insets_Ic1' Outsets_Ic1'.
               clear -Hc4 S_sub_c1; set_solver.
+            - rewrite Insets_Ic1'. intros k'. rewrite elem_of_difference.
+              intros [Hk1' Hk2']. by apply Hc5.
             - admit.
             - admit. }
+          iAssert (hist γ_t γ_m M1' (T1+1))%I with "[Hist]" as "Hist".
+          { admit. }
+          iAssert (▷ helping_inv N γ_t γ_r γ_td1 γ_td2 γ_ght M1')%I with
+            "[Help]" as "Help".
+          { admit. }
+          iAssert (past_state γ_m t0 s1')%I as "Past_s1'".
+          { admit. }
+          assert (FP s1' = FP s1) as FP_s1'.
+          { by rewrite /FP /s1' Hs1. }
+          assert (abs s1' = abs s1) as Habs'.
+          { by rewrite /abs /s1' Hs1. }
+          iAssert (dsRepI γ_r (abs s1'))%I with "[Ds]" as "Ds".
+          { by rewrite Habs'. }
+          iAssert (own γ_ks (● prodKS (KS, abs s1')))%I with "[GKS]" as "GKS".
+          { by rewrite Habs'. }
+          assert (∀ n, n ≠ p → Next s1' n = Next s1 n) as HN.
+          { intros n Hnc. 
+            rewrite /Next /s1' Hs1 /= /Nx1' lookup_insert_ne; try done. }
+          assert (Next s1' p = <[0:=cn]> (Next s1 p)) as HNp.
+          { by rewrite /s1' Hs1 /Next /Nx1' lookup_insert Def_next' /Next Hs1. }
+          assert (∀ n, Key s1' n = Key s1 n) as HK.
+          { by rewrite /Key /s1' Hs1 /=. }
+          assert (∀ n, n ≠ p → n ≠ c → FI s1' n = FI s1 n) as HI.
+          { intros n Hnp Hnc. rewrite /FI /s1' /I1' Hs1 /= !lookup_insert_ne.
+            all: done. }
+          assert (FI s1' p = Ip1') as HIp.
+          { rewrite /FI /s1' /I1' lookup_insert_ne; try done. 
+            by rewrite lookup_insert. }
+          assert (FI s1' c = Ic1') as HIc.
+          { rewrite /FI /s1' /I1' lookup_insert; try done. }
+          assert (∀ n, Mark s1' n = Mark s1 n) as HM.
+          { by rewrite /FI /s1' Hs1. }
+          assert (∀ n, Height s1' n = Height s1 n) as HT.
+          { by rewrite /FI /s1' Hs1. }
+          iAssert (⌜snapshot_constraints s1'⌝)%I as "SShot1'".
+          { iPureIntro. exists FP1, C1, Ht1, Mk1, Nx1', Ky1, I1'.
+            repeat split; try done.
+            rewrite /Nx1'. rewrite dom_insert_L.
+            assert (p ∈ dom Nx1) as H'. 
+            { rewrite Hs1 in FP_p1. rewrite Dom_Nx1. by unfold FP in FP_p1. }
+            clear -H' Dom_Nx1. set_solver.
+            rewrite /I1' !dom_insert_L.
+            assert ({[p;c]} ⊆ dom I1) as H'.
+            { rewrite Hs1 /FP -Dom_I1 in FP_p1 FP_c1. 
+              clear -FP_c1 FP_p1; set_solver. }
+            clear -H' Dom_I1; set_solver. }
+          assert (p ≠ tl) as p_neq_tl. admit.
+          assert (per_tick_inv s1') as PT_s1'.
+          { destruct PT_s1 as (PT1'&PT2'&PT3'&PT4'&PT5'&PT6').
+            split; last split; last split; last split; last split.
+            - destruct PT1' as (PT11'&PT12'&PT13'&PT14'&PT15'). repeat split.
+              + intros i'. rewrite /Marki HM. apply PT11'.
+              + rewrite HK. apply PT12'.
+              + rewrite HK. apply PT13'.
+              + by rewrite FP_s1'.
+              + by rewrite FP_s1'.
+            - rewrite /s1' /GFI /FP /FI. admit.
+            - intros n Hn. rewrite FP_s1' in Hn. apply PT3' in Hn.
+              destruct (decide (n = p)) as [-> | Hnp].
+              + rewrite HNp HK HIp HM HT.
+                destruct Hn as (Hn1&Hn2&Hn3&Hn4&Hn5&Hn6&Hn7).
+                split; last split; last split; last split; last split; 
+                  last split; try done.
+                * intros i'. destruct (decide (i' = 0)) as [-> | Hi'i].
+                  rewrite lookup_insert. split; try done.
+                  rewrite lookup_insert_ne; try done.
+                * rewrite dom_insert_L Hn3. admit.
+                * rewrite lookup_insert Mark_p1. done.
+              + destruct (decide (n = c)) as [-> | Hnc]; last first.
+                { rewrite HK HM HT. rewrite HN; try done. rewrite HI; try done. }
+                rewrite HK HM HT HIc HN; try done.
+                destruct Hn as (Hn1&Hn2&Hn3&Hn4&Hn5&Hn6&Hn7).
+                split; last split; last split; last split; last split; last split;
+                  try done. rewrite Mark_c1 Next_c1. done.
+            - intros n1 n2 i'. destruct (decide (n1 = p)) as [-> | Hn1p].
+              + rewrite /Nexti HNp !HK. destruct (decide (i' = 0)) as [-> | Hi'i].
+                rewrite lookup_insert. intros [=<-]. admit.
+                rewrite lookup_insert_ne; try done. apply PT4'.
+              + rewrite !HK /Nexti HN; try done. apply PT4'. 
+            - intros n1 n2 i'. rewrite FP_s1'. 
+              destruct (decide (n1 = p)) as [-> | Hn1p].
+              + rewrite /Nexti HNp. destruct (decide (i' = 0)) as [-> | Hi'i].
+                rewrite lookup_insert. intros [=<-]. admit.
+                rewrite lookup_insert_ne; try done. apply PT5'.
+              + rewrite /Nexti HN; try done. apply PT5'.
+            - admit. }
+          assert (transition_inv s1 s1') as Trans_s1.
+          { repeat split; try rewrite FP_s1'; try done; last first.
+            - intros n i' Hfp. rewrite /Marki HM. done.
+            - intros n. rewrite /Marki HM. intros H' H''. 
+              rewrite H' in H''; try done.
+            - intros n' i' Hn'. destruct (decide (n' = p)) as [-> | Hnp].
+              + rewrite /Marki HM /Nexti HNp. 
+                destruct (decide (i' = 0)) as [-> | Hi].
+                rewrite Mark_p1. clear; try done.
+                rewrite lookup_insert_ne; try done.
+              + rewrite /Marki /Nexti HM HN; try done. }
+          iAssert (resources γ_ks s1')%I 
+            with "[GKS Nodes_KS Node_p Nodes_rest]" as "Res".
+          { iFrame "GKS". rewrite FP_s1'. iSplitR "Nodes_KS".
+            rewrite (big_opS_delete _ (FP s1) p); try done.
+            iSplitL "Node_p". rewrite Def_next' HNp HM HK HT. done.
+            iApply (big_sepS_mono with "Nodes_rest"); try done.
+            intros x Hx. iIntros "Hn". rewrite HK HM HT HN. done.
+            clear -Hx; set_solver.
+            iApply (big_sepS_mono with "Nodes_KS"); try done.
+            intros x Hx. iIntros "Hn". admit. 
+            (*
+            assert (Content s1' x = Content s1 x) as ->.
+            rewrite /Content HK /Marki HM. done. done.*) }
 
-        * iDestruct "SShot1" as %[FP1 [C1 [Mk1 [Nx1 [Ky1 [I1 
-            [Hs1 [Dom_Mk1 [Dom_Nx1 [Dom_Ky1 Dom_I1]]]]]]]]]].
+          iAssert (∃ s, past_state γ_m t0 s ∗ ⌜traversal_inv s 0 k p cn⌝)%I 
+            as "#HtrInv'".
+          { iExists s1'. iFrame "#". iPureIntro. repeat split.
+            rewrite FP_s1'; try done. admit. rewrite HK.
+            admit. rewrite /Marki HM Mark_p1. done. rewrite /Nexti HNp.
+            by rewrite lookup_insert. admit. admit. }  
+          iModIntro. iSplitR "Hpost".
+          { iNext. iExists M1', (T1+1), s1'. iFrame "∗#%".
+            iPureIntro; rewrite /M1'; split; last split.
+            - by rewrite lookup_total_insert.
+            - intros t Ht. destruct (decide (t = T1+1)) as [-> | Ht'].
+              + by rewrite lookup_total_insert.
+              + rewrite lookup_total_insert_ne; try done. apply PT1.
+                rewrite dom_insert in Ht. clear -Ht' Ht; set_solver.
+            - intros t Ht. destruct (decide (t = T1)) as [-> | Ht'].
+              + rewrite lookup_total_insert. rewrite lookup_total_insert_ne.
+                apply leibniz_equiv in Habs1. by rewrite Habs1. clear; lia.
+              + rewrite !lookup_total_insert_ne. apply Trans_M1.
+                all: clear -Ht Ht'; lia. }
+          wp_pures.
+          iApply "IH"; try done.
+        * iDestruct "SShot1" as %[FP1 [C1 [Ht1 [Mk1 [Nx1 [Ky1 [I1 
+            [Hs1 [Dom_Ht1 [Dom_Mk1 [Dom_Nx1 [Dom_Ky1 Dom_I1]]]]]]]]]]]].
           set Nx1' := <[p := next']> Nx1.
-          set s1' := (FP1, C1, Mk1, Nx1', Ky1, I1): snapshot.
+          set s1' := (FP1, C1, Ht1, Mk1, Nx1', Ky1, I1): snapshot.
           set M1' := <[T1 + 1 := s1']> M1.
           iAssert (⌜per_tick_inv s1⌝)%I as %PT_s1.
           { iDestruct "Hist" as (M')"(_&_&_&%&_)". iPureIntro.
@@ -372,19 +564,21 @@ Module SKIPLIST1_SPEC_TRAVERSE.
           { by rewrite /FI /s1' Hs1 /=. }
           assert (∀ n, Mark s1' n = Mark s1 n) as HM.
           { by rewrite /FI /s1' Hs1. }
+          assert (∀ n, Height s1' n = Height s1 n) as HT.
+          { by rewrite /FI /s1' Hs1. }
           assert (p ≠ tl) as p_neq_tl. admit.
           assert (Key s1 p < Key s1 cn) as Key_pcn. admit.
           assert (cn ∈ FP s1) as FP_cn1. admit.
           iAssert (⌜snapshot_constraints s1'⌝)%I as "SShot1'".
-          { iPureIntro. exists FP1, C1, Mk1, Nx1', Ky1, I1.
+          { iPureIntro. exists FP1, C1, Ht1, Mk1, Nx1', Ky1, I1.
             repeat split; try done.
             rewrite /Nx1'. rewrite dom_insert_L.
             assert (p ∈ dom Nx1). 
             { rewrite Hs1 in FP_p1. rewrite Dom_Nx1. by unfold FP in FP_p1. }
             clear -H Dom_Nx1. set_solver. }
           assert (per_tick_inv s1') as PT_s1'.
-          { destruct PT_s1 as (PT1'&PT2'&PT3'&PT4'&PT5').
-            split; last split; last split; last split.
+          { destruct PT_s1 as (PT1'&PT2'&PT3'&PT4'&PT5'&PT6').
+            split; last split; last split; last split; last split.
             - destruct PT1' as (PT11'&PT12'&PT13'&PT14'&PT15'). repeat split.
               + intros i'. rewrite /Marki HM. apply PT11'.
               + rewrite HK. apply PT12'.
@@ -394,15 +588,16 @@ Module SKIPLIST1_SPEC_TRAVERSE.
             - rewrite /s1' /GFI /FP /FI. by rewrite Hs1 /GFI /FP /FI in PT2'.
             - intros n Hn. rewrite FP_s1' in Hn. apply PT3' in Hn.
               destruct (decide (n = p)) as [-> | Hnp].
-              + rewrite HNp HK HI HM.
-                destruct Hn as (Hn1&Hn2&Hn3&Hn4&Hn5&Hn6).
-                split; last split; last split; last split; last split; try done.
+              + rewrite HNp HK HI HT HM.
+                destruct Hn as (Hn1&Hn2&Hn3&Hn4&Hn5&Hn6&Hn7).
+                split; last split; last split; last split; last split; 
+                  last split; try done.
                 * intros i'. destruct (decide (i' = i)) as [-> | Hi'i].
                   rewrite lookup_insert. split; try done.
                   rewrite lookup_insert_ne; try done.
-                * rewrite dom_insert. clear -Hn3; set_solver.
+                * rewrite dom_insert_L Hn3. admit.
                 * rewrite lookup_insert_ne; try done.
-              + rewrite HK HI HM. rewrite HN; try done.
+              + rewrite HK HT HI HM. rewrite HN; try done.
             - intros n1 n2 i'. destruct (decide (n1 = p)) as [-> | Hn1p].
               + rewrite /Nexti HNp !HK. destruct (decide (i = i')) as [-> | Hi'i].
                 rewrite lookup_insert. intros [=<-]. done. 
@@ -413,19 +608,26 @@ Module SKIPLIST1_SPEC_TRAVERSE.
               + rewrite /Nexti HNp. destruct (decide (i = i')) as [-> | Hi'i].
                 rewrite lookup_insert. intros [=<-]. done. 
                 rewrite lookup_insert_ne; try done. apply PT5'.
-              + rewrite /Nexti HN; try done. apply PT5'. }
+              + rewrite /Nexti HN; try done. apply PT5'.
+            - admit. }
           assert (transition_inv s1 s1') as Trans_s1.
           { repeat split; try rewrite FP_s1'; try done; last first.
             - intros n i' Hfp. rewrite /Marki HM. done.
             - intros n. rewrite /Marki HM. intros H' H''. 
-              rewrite H' in H''; try done. }
+              rewrite H' in H''; try done.
+            - intros n' i' Hn'. destruct (decide (n' = p)) as [-> | Hnp].
+              + rewrite /Marki HM /Nexti HNp. 
+                destruct (decide (i' = i)) as [-> | Hi].
+                rewrite Mark_p1. clear; try done.
+                rewrite lookup_insert_ne; try done.
+              + rewrite /Marki /Nexti HM HN; try done. }
           iAssert (resources γ_ks s1')%I 
             with "[GKS Nodes_KS Node_p Nodes_rest]" as "Res".
           { iFrame "GKS". rewrite FP_s1'. iSplitR "Nodes_KS".
             rewrite (big_opS_delete _ (FP s1) p); try done.
-            iSplitL "Node_p". rewrite Def_next' HNp HM HK. done.
+            iSplitL "Node_p". rewrite Def_next' HNp HT HM HK. done.
             iApply (big_sepS_mono with "Nodes_rest"); try done.
-            intros x Hx. iIntros "Hn". rewrite HK HM HN. done.
+            intros x Hx. iIntros "Hn". rewrite HK HT HM HN. done.
             clear -Hx; set_solver.
             iApply (big_sepS_mono with "Nodes_KS"); try done.
             intros x Hx. iIntros "Hn". rewrite HI.
@@ -437,7 +639,7 @@ Module SKIPLIST1_SPEC_TRAVERSE.
           { iExists s1'. iFrame "#". iPureIntro. repeat split.
             rewrite FP_s1'; try done. rewrite FP_s1'; try done.
             admit. rewrite /Marki HM Mark_p1. done. rewrite /Nexti HNp.
-            by rewrite lookup_insert. }  
+            by rewrite lookup_insert. admit. admit. }  
           iModIntro. iSplitR "Hpost".
           { iNext. iExists M1', (T1+1), s1'. iFrame "∗#%".
             iPureIntro; rewrite /M1'; split; last split.
@@ -555,8 +757,11 @@ Module SKIPLIST1_SPEC_TRAVERSE.
     { (* interpolation *) admit. }
     rewrite (big_sepS_delete _ (FP s0) p); last by eauto.
     iDestruct "Nodes" as "(Node_p & Nodes_rest)".
-    iAaccIntro with "Node_p".
-    { iIntros "Node_p". iModIntro. iFrame "Hpost Hpreds Hsuccs Hj".
+    iAssert ((node p (Height s0 p) (Mark s0 p) (Next s0 p) (Key s0 p)) 
+      ∗ ⌜i < Height s0 p⌝)%I with "[Node_p]" as "Hpre".
+    { admit. }
+    iAaccIntro with "Hpre".    
+    { iIntros "(Node_p&_)". iModIntro. iFrame "Hpost Hpreds Hsuccs Hj".
       iNext; iExists M0, T0, s0. iFrame "∗%#". 
       rewrite (big_sepS_delete _ (FP s0) p); last by eauto. iFrame. }
     iIntros (m c) "(Node_p & %Mark_p0 & %Next_p0)".
@@ -621,7 +826,7 @@ Module SKIPLIST1_SPEC_TRAVERSE.
     iFrame "∗#". iIntros (ores ps ss b)"Hores".
     destruct ores as [[[preds' succs'] res] |]; last first.
     { wp_pures. iDestruct "Hores" as "(Hpreds & Hsuccs)".
-      iApply ("IH" with "[Hpreds Hsuccs]"). iFrame. iIntros (j)"%Hj".
+      iApply ("IH" with "[Hpreds Hsuccs]"); try iFrame. iIntros (j)"%Hj".
       assert (j = L-1) as -> by lia. admit. }
     wp_pures. iDestruct "Hores" as "(%H' & %H'' & %H1' & H1'')". 
     rewrite /= in H' H'' H1'. subst preds' succs' b.  
