templates/lockfree/maintenanceOp_delete.v
@@ -1,0 +1,303 @@
+(* Herlihy Skiplist with a single level : Delete *)
+
+From iris.algebra Require Import excl auth cmra gmap agree gset numbers.
+From iris.algebra.lib Require Import dfrac_agree.
+From iris.heap_lang Require Export notation locations lang.
+From iris.base_logic.lib Require Export invariants.
+From iris.program_logic Require Export atomic.
+From iris.proofmode Require Import tactics.
+From iris.heap_lang Require Import proofmode par.
+From iris.heap_lang.lib Require Import nondet_bool.
+From iris.bi.lib Require Import fractional.
+Set Default Proof Using "All".
+From iris.bi.lib Require Import fractional.
+Require Export skiplist_v1_util list_flow_upd_marking.
+
+Module MAINTENANCEOP_DELETE.
+  Import SKIPLIST1 SKIPLIST1_UTIL.DEFS SKIPLIST1_UTIL.
+
+  Parameter markNode_spec : ∀ (n: Node) (i: nat),
+    ⊢  <<< ∀∀ h mark next k, node n h mark next k ∗ ⌜i < h⌝ >>>
+            markNode #n #i @⊤
+      <<< ∃∃ (success: bool) mark',
+              node n h mark' next k
+            ∗ (match success with true => ⌜mark !!! i = false
+                                            ∧ mark' = <[i := true]> mark⌝
+                                | false => ⌜mark !!! i = true
+                                            ∧ mark' = mark⌝ end),
+              RET (match success with true => SOMEV #() 
+                                    | false => NONEV end)  >>>.
+
+  Parameter getHeight_spec : ∀ (n: Node) (i: nat),
+    ⊢ <<< ∀∀ h mark next k, node n h mark next k >>>
+          getHeight #n @⊤
+      <<< node n h mark next k, RET #h >>>.
+
+  Parameter permute_levels_spec : ∀ (L: nat),
+        {{{ True }}}
+           permute_levels #L
+        {{{ (perm: loc) (vs: list val) (xs: list nat), RET #perm;
+              perm ↦∗ vs
+            ∗ ⌜vs = (fun n => # (LitInt (Z.of_nat n))) <$> xs⌝
+            ∗ ⌜xs ≡ₚ seq 1 (L-1)⌝ }}}.
+
+  Lemma maintenanceOp_delete_rec_spec N γ_t γ_s γ_m γ_td1 γ_td2 γ_ght t0 c
+    perm vs xs i h:
+      main_inv N γ_t γ_s γ_m γ_td1 γ_td2 γ_ght -∗
+        {{{   perm ↦∗ vs
+            ∗ ⌜vs = (fun n => # (LitInt (Z.of_nat n))) <$> xs⌝
+            ∗ ⌜xs ≡ₚ seq 1 (h-1)⌝
+            ∗ (∃ s, past_state γ_m t0 s ∗ ⌜c ∈ FP s⌝ ∗ ⌜h = Height s c⌝
+                    ∗ ⌜∀ j, j < i → Marki s c (xs !!! j) = true⌝) }}}
+           maintenanceOp_delete_rec #i #h #perm #c
+        {{{ RET #();
+              (∃ s, past_state γ_m t0 s ∗ ⌜c ∈ FP s⌝ ∗ ⌜h = Height s c⌝
+                    ∗ ⌜∀ j, j < h-1 → Marki s c (xs !!! j) = true⌝)
+            ∗ perm ↦∗ vs }}}.
+  Proof.
+    iIntros "#HInv". iLöb as "IH" forall (i).
+    iIntros (Φ) "!# (Hperm & %Def_vs & %Perm_xs & #Hmark) Hpost". 
+    wp_lam. wp_pures.
+    destruct (bool_decide (Z.lt i (h - 1)%Z)) eqn: Hbool; wp_pures.
+    - rewrite bool_decide_eq_true in Hbool.
+      assert (is_Some (xs !! i)) as [idx Hidx].
+      { assert (i < length xs) as H'. rewrite Perm_xs seq_length. lia.
+        by rewrite lookup_lt_is_Some. }
+      wp_apply (wp_load_offset _ _ _ (DfracOwn 1) (i) (vs) #idx
+        with "[Hperm]"); try done.
+      { rewrite Def_vs. rewrite list_lookup_fmap. rewrite Hidx.
+        by simpl. }
+      iIntros "Hperm". wp_pures.
+      awp_apply markNode_spec; try done.
+      iInv "HInv" as (M0 T0 s0) "(>Ds & >%Habs0 & >Hist & Help & >Templ)".
+      { admit. }
+      iDestruct "Templ" as "(SShot0 & Res & %PT0 & %Trans_M0)".
+      iDestruct "Res" as "(GKS & Nodes & Nodes_KS)".
+      iAssert (⌜c ∈ FP s0⌝)%I as %FP_c0.
+      { (* interpolation *) admit. }
+      rewrite (big_sepS_delete _ (FP s0) c); last by eauto.
+      iDestruct "Nodes" as "(Node_c & Nodes_rest)".
+      iAssert ((node c (Height s0 c) (Mark s0 c) (Next s0 c) (Key s0 c)) 
+        ∗ ⌜idx < Height s0 c⌝)%I with "[Node_c]" as "Hpre".
+      { admit. }
+      iAaccIntro with "Hpre".
+      { iIntros "(Node_c & _)". iModIntro. iFrame "Hpost".
+        iSplitR "Hperm"; try done. iNext; iExists M0, T0, s0. iFrame "∗%#". 
+        rewrite (big_sepS_delete _ (FP s0) c); try done. iFrame. }
+      iIntros (success mark')"(Node_c & Hif)". destruct success.
+      + iDestruct "Hif" as %[Mark_c0 Def_mark'].
+        iDestruct "SShot0" as %[FP0 [C0 [Ht0 [Mk0 [Nx0 [Ky0 [I0 
+          [Hs0 [Dom_Ht0 [Dom_Mk0 [Dom_Nx0 [Dom_Ky0 Dom_I0]]]]]]]]]]]].
+        set Mk0' := <[c := mark']> Mk0.
+        set s0' := (FP0, C0, Ht0, Mk0', Nx0, Ky0, I0): snapshot.
+        set M0' := <[T0 + 1 := s0']> M0.
+        iAssert (⌜per_tick_inv s0⌝)%I as %PT_s0.
+        { iDestruct "Hist" as (M')"(_&_&_&%&_)". iPureIntro.
+          apply leibniz_equiv in Habs0. rewrite <-Habs0.
+          by apply PT0. }
+        iAssert (hist γ_t γ_m M0' (T0+1))%I with "[Hist]" as "Hist".
+        { admit. }
+        iAssert (▷ helping_inv N γ_t γ_s γ_td1 γ_td2 γ_ght M0')%I with
+          "[Help]" as "Help".
+        { admit. }
+        iAssert (past_state γ_m t0 s0')%I as "Past_s0'".
+        { admit. } 
+        iAssert (∃ s : snapshot, past_state γ_m t0 s ∗ ⌜c ∈ FP s⌝ ∗ ⌜h = Height s c⌝
+          ∗ ⌜∀ j : nat, j < i + 1 → Marki s c (xs !!! j) = true⌝)%I as "#Hmark'".
+        { iDestruct "Hmark" as (s) "(Hpast_s & %FP_c' & %Ht_c & %Hj)".
+          assert (∀ j, j < i → Marki s0 c (xs !!! j) = true) as Hj0.
+          { admit. }
+          iAssert (⌜Marki s0' c (xs !!! i) = true⌝)%I as %Hi.
+          { iPureIntro. rewrite list_lookup_total_alt Hidx /=.
+            rewrite /s0' /Marki /Mark /Mk0' lookup_insert Def_mark'.
+            by rewrite lookup_total_insert. }
+          iExists s0'. iFrame "Past_s0'". iPureIntro.
+          split. rewrite /s0' /FP. by rewrite Hs0 /FP in FP_c0.
+          split. admit.
+          intros j Hj'. destruct (decide (j = i)) as [-> | Hji]; try done.
+          rewrite /s0' /Marki /Mark /Mk0' lookup_insert Def_mark'.
+          rewrite lookup_total_insert_ne. rewrite /Marki in Hj0.
+          apply Hj0. lia. 
+          clear -Hji Hj' Hidx Hbool Perm_xs. intros H'. apply Hji.
+          assert (is_Some (xs !! j)) as [idx' Hidx'].
+          apply lookup_lt_is_Some. rewrite Perm_xs seq_length. lia.
+          assert (idx' = idx) as ->.
+          apply lookup_total_correct in Hidx'. rewrite -Hidx'. admit.
+          assert (NoDup xs) as H''. rewrite Perm_xs. apply NoDup_seq.
+          by pose proof NoDup_lookup xs i j idx H'' Hidx Hidx'. }
+        assert (FP s0' = FP s0) as FP_s0'.
+        { by rewrite /FP /s0' Hs0. }
+        assert (abs s0' = abs s0) as Habs'.
+        { by rewrite /abs /s0' Hs0. }
+        iAssert (dsRepI γ_s (abs s0'))%I with "[Ds]" as "Ds".
+        { by rewrite Habs'. }
+        iAssert (own γ_ks (● prodKS (KS, abs s0')))%I with "[GKS]" as "GKS".
+        { by rewrite Habs'. }
+        assert (idx ≠ 0) as Hidx0.
+        { intros ->. assert (0 ∈ seq 1 (h-1)) as H'.
+          rewrite -Perm_xs. rewrite elem_of_list_lookup.
+          by exists i. rewrite elem_of_seq in H'.
+          clear -H'; lia. }
+        assert (∀ n, Next s0' n = Next s0 n) as HN.
+        { by rewrite /Next /s0' Hs0 /=. }
+        assert (∀ n, Height s0' n = Height s0 n) as HT.
+        { by rewrite /s0' Hs0 /=. }
+        assert (∀ n, Key s0' n = Key s0 n) as HK.
+        { by rewrite /Key /s0' Hs0 /=. }
+        assert (∀ n, FI s0' n = FI s0 n) as HI.
+        { by rewrite /FI /s0' Hs0 /=. }
+        assert (∀ n, n ≠ c → Mark s0' n = Mark s0 n) as HM.
+        { intros n Hnc. by rewrite /FI /s0' Hs0 /Mk0' /= lookup_insert_ne. }
+        assert (Mark s0' c = <[idx := true]> (Mark s0 c)) as HMc.
+        { rewrite /FI /s0' Hs0 /Mk0' /= lookup_insert Def_mark'.
+          by rewrite Hs0 /Mark. }
+        assert (c ≠ hd) as c_neq_hd. admit.
+        assert (c ≠ tl) as c_neq_tl. admit.
+        iAssert (⌜snapshot_constraints s0'⌝)%I as "SShot0'".
+        { iPureIntro. exists FP0, C0, Ht0, Mk0', Nx0, Ky0, I0.
+          repeat split; try done.
+          rewrite /Mk0'. rewrite dom_insert_L.
+          assert (c ∈ dom Mk0). 
+          { rewrite Hs0 in FP_c0. rewrite Dom_Mk0. by unfold FP in FP_c0. }
+          clear -H Dom_Mk0. set_solver. }
+        assert (per_tick_inv s0') as PT_s0'.
+        { destruct PT_s0 as (PT1&PT2&PT3&PT4&PT5&PT6).
+          split; last split; last split; last split; last split.
+          - destruct PT1 as (PT11&PT12&PT13&PT14&PT15). repeat split.
+            + intros i'. rewrite /Marki /Mark /s0' /Mk0' lookup_insert_ne; try done.
+              rewrite /Marki /Mark Hs0 in PT11. apply PT11.
+            + rewrite /Key /s0'. by rewrite /Key Hs0 in PT12.
+            + rewrite /Key /s0'. by rewrite /Key Hs0 in PT13.
+            + by rewrite FP_s0'.
+            + by rewrite FP_s0'.
+          - rewrite /s0' /GFI /FP /FI. by rewrite Hs0 /GFI /FP /FI in PT2.
+          - intros n Hn. rewrite FP_s0' in Hn. apply PT3 in Hn.
+            destruct (decide (n = c)) as [-> | Hnc].
+            + rewrite HT HN HK HI HMc.
+              destruct Hn as (Hn1&Hn2&Hn3&Hn4&Hn5&Hn6&Hn7).
+              split; last split; last split; last split; last split; 
+                last split; try done.
+              * intros [i' Hi']. destruct (decide (i' = idx)) as [-> | Hi].
+                by rewrite lookup_total_insert in Hi'.
+                rewrite lookup_total_insert_ne in Hi'; try done.
+                rewrite lookup_total_insert_ne; try done. apply Hn1.
+                exists i'; try done.
+              * admit.
+              * rewrite lookup_total_insert_ne; try done.
+            + rewrite HT HN HK HI HM; try done.
+          - intros n1 n2 i'. rewrite /Nexti. rewrite HN !HK. apply PT4.
+          - intros n1 n2 i'. rewrite /Nexti. rewrite HN FP_s0'. apply PT5.
+          - intros n1 n2 i'. rewrite /Nexti HT. admit. }
+        assert (transition_inv s0 s0') as Trans_s0.
+        { repeat split; try rewrite FP_s0'; try done; last first.
+          intros n i' Hn; rewrite /Marki; intros Hm.
+          destruct (decide (n = c)) as [-> | Hnc].
+          - rewrite HMc. destruct (decide (i' = idx)) as [-> | Hi'].
+            + by rewrite lookup_total_insert.
+            + by rewrite lookup_total_insert_ne.
+          - by rewrite HM.
+          - admit.
+          - admit. }
+        iAssert (resources γ_ks s0')%I 
+          with "[GKS Nodes_KS Node_c Nodes_rest]" as "Res".
+        { iFrame "GKS". rewrite FP_s0'. iSplitR "Nodes_KS".
+          rewrite (big_opS_delete _ (FP s0) c).
+          iSplitL "Node_c". rewrite Def_mark' HT HMc HN HK. done.
+          iApply (big_sepS_mono with "Nodes_rest"); try done.
+          intros x Hx. iIntros "Hn". rewrite HN HT HK HM. done.
+          clear -Hx; set_solver. done. 
+          iApply (big_sepS_mono with "Nodes_KS"); try done.
+          intros x Hx. iIntros "Hn". rewrite HI.
+          assert (Content s0' x = Content s0 x) as ->.
+          rewrite /Content HK. destruct (decide (x = c)) as [-> | Hxc].
+          rewrite /Marki HMc lookup_total_insert_ne; try done.
+          rewrite /Marki HM; try done. done. }
+        iModIntro. iSplitR "Hperm Hpost".
+        { iNext. iExists M0', (T0+1), s0'. iFrame "∗#%".
+          iPureIntro; rewrite /M0'; split; last split.
+          - by rewrite lookup_total_insert.
+          - intros t Ht. destruct (decide (t = T0+1)) as [-> | Ht'].
+            + by rewrite lookup_total_insert.
+            + rewrite lookup_total_insert_ne; try done. apply PT0.
+              rewrite dom_insert in Ht. clear -Ht' Ht; set_solver.
+          - intros t Ht. destruct (decide (t = T0)) as [-> | Ht'].
+            + rewrite lookup_total_insert. rewrite lookup_total_insert_ne.
+              apply leibniz_equiv in Habs0. by rewrite Habs0. clear; lia.
+            + rewrite !lookup_total_insert_ne. apply Trans_M0.
+              all: clear -Ht Ht'; lia. }
+        wp_pures.
+        iSpecialize ("IH" $! (i+1)).
+        assert (Z.of_nat (i+1) = (Z.of_nat i + 1)%Z) as H' by lia.
+        iEval (rewrite H') in "IH". iApply ("IH" with "[Hperm]"); try done.
+        iFrame "Hperm Hmark' %".
+      + iDestruct "Hif" as %[Mark_c0 ->].
+        iAssert (∃ s : snapshot, past_state γ_m t0 s ∗ ⌜c ∈ FP s⌝ ∗ ⌜h = Height s c⌝
+          ∗ ⌜∀ j : nat, j < i + 1 → Marki s c (xs !!! j) = true⌝)%I as "#Hmark'".
+        { assert (∀ j, j < i → Marki s0 c (xs !!! j) = true) as Hj0.
+          { admit. }
+          iAssert (⌜Marki s0 c (xs !!! i) = true⌝)%I as %Hi.
+          { iPureIntro. rewrite list_lookup_total_alt Hidx /=. done. }
+          iExists s0. iSplitL. iExists T0. admit.
+          iPureIntro; split; try done. split. admit.
+          intros j Hj. destruct (decide (j = i)) as [-> | Hji]; try done.
+          apply Hj0. lia. }
+        iModIntro. iSplitR "Hperm Hpost".
+        { iNext. iExists M0, T0, s0. iFrame "∗#%".
+          rewrite (big_opS_delete _ (FP s0) c); try done.
+          iFrame "Nodes_rest". iFrame. }
+        wp_pures.
+        iSpecialize ("IH" $! (i+1)).
+        assert (Z.of_nat (i+1) = (Z.of_nat i + 1)%Z) as H' by lia.
+        iEval (rewrite H') in "IH". iApply ("IH" with "[Hperm]"); try done.
+        iFrame "Hperm Hmark' %".
+    - rewrite bool_decide_eq_false in Hbool.
+      iApply "Hpost". iFrame "Hperm". 
+      iDestruct "Hmark" as (s) "(Hpast_s & %FP_c' & %HT_c & %Hj)".
+      iModIntro. iExists s. iFrame "#%". iPureIntro.
+      intros j Hj'. apply Hj. lia.
+  Admitted.
+
+    
+  Lemma maintenanceOp_delete_spec N γ_t γ_s γ_m γ_td1 γ_td2 γ_ght t0 c:
+      main_inv N γ_t γ_s γ_m γ_td1 γ_td2 γ_ght -∗
+        {{{ ∃ s, past_state γ_m t0 s ∗ ⌜c ∈ FP s⌝ }}}
+           maintenanceOp_delete #c
+        {{{ RET #();
+              (∃ s h, past_state γ_m t0 s ∗ ⌜c ∈ FP s⌝ ∗ ⌜h = Height s c⌝
+                    ∗ ⌜∀ i, 1 ≤ i < h → Marki s c i = true⌝) }}}.
+  Proof.
+    iIntros "#HInv". iIntros (Φ) "!# #FP_c Hpost".
+    wp_lam. wp_pures. awp_apply getHeight_spec; try done. 
+    iInv "HInv" as (M0 T0 s0) "(>Ds & >%Habs0 & >Hist & Help & >Templ)".
+    { admit. }
+    iDestruct "Templ" as "(SShot0 & Res & %PT0 & %Trans_M0)".
+    iDestruct "Res" as "(GKS & Nodes & Nodes_KS)".
+    iAssert (⌜c ∈ FP s0⌝)%I as %FP_c0.
+    { (* interpolation *) admit. }
+    rewrite (big_sepS_delete _ (FP s0) c); last by eauto.
+    iDestruct "Nodes" as "(Node_c & Nodes_rest)".
+    iAaccIntro with "Node_c".
+    { iIntros "Node_c". iModIntro. iFrame "Hpost".
+      iNext; iExists M0, T0, s0. iFrame "∗%#". 
+      rewrite (big_sepS_delete _ (FP s0) c); try done. iFrame. }
+    iIntros "Node_c". iSplitR " Hpost".
+    { iModIntro. iNext; iExists M0, T0, s0. iFrame "∗%#". 
+      rewrite (big_sepS_delete _ (FP s0) c); try done. iFrame. }  
+    iModIntro. wp_pures. set h := Height s0 c. 
+    wp_apply permute_levels_spec; try done.
+    iIntros (perm vs xs)"(Hperm & %Def_vs & %Perm_xs)". wp_pures. 
+    wp_apply (maintenanceOp_delete_rec_spec with "[] [Hperm]"); try done.
+    { iFrame "Hperm %". iDestruct "FP_c" as (s)"(Hs & FP_c)".
+      iExists s. iFrame "Hs FP_c". iPureIntro; split; try lia. admit. }
+    iIntros "(Hs & Hperm)". iDestruct "Hs" as (s)"(Hs & %H' & %H'' & %H1')".
+    iApply "Hpost". iExists s, h; iFrame. iPureIntro; repeat split; try done.
+    intros i Hi. assert (∃ j, j < h - 1 ∧ (xs !!! j = i)) as [j [H1'' <-]].
+    { assert (i ∈ xs) as Hixs. rewrite Perm_xs elem_of_seq. lia.
+      rewrite elem_of_list_lookup in Hixs. destruct Hixs as [j Hjxs].
+      exists j; split. apply lookup_lt_Some in Hjxs. 
+      by rewrite Perm_xs seq_length in Hjxs. 
+      by rewrite list_lookup_total_alt Hjxs.  }
+    apply H1'; try done.
+  Admitted.
+
+End MAINTENANCEOP_DELETE.
