templates/lockfree/maintenanceOp_insert.v
@@ -1,0 +1,151 @@
+(* Herlihy Skiplist with a single level : Insert *)
+
+From iris.algebra Require Import excl auth cmra gmap agree gset numbers.
+From iris.algebra.lib Require Import dfrac_agree.
+From iris.heap_lang Require Export notation locations lang.
+From iris.base_logic.lib Require Export invariants.
+From iris.program_logic Require Export atomic.
+From iris.proofmode Require Import tactics.
+From iris.heap_lang.lib Require Import nondet_bool.
+From iris.heap_lang Require Import proofmode par.
+From iris.bi.lib Require Import fractional.
+Set Default Proof Using "All".
+From iris.bi.lib Require Import fractional.
+From flows Require Export skiplist_v1_util list_flow_upd_insert.
+
+Module MAINTENANCEOP_INSERT.
+  Import SKIPLIST1 SKIPLIST1_UTIL.DEFS SKIPLIST1_UTIL.
+
+  Parameter permute_levels_spec : ∀ (L: nat),
+        {{{ True }}}
+           permute_levels #L
+        {{{ (perm: loc) (vs: list val) (xs: list nat), RET #perm;
+              perm ↦∗ vs
+            ∗ ⌜vs = (fun n => # (LitInt (Z.of_nat n))) <$> xs⌝
+            ∗ ⌜xs ≡ₚ seq 1 (L-1)⌝ }}}.
+
+  Parameter getHeight_spec : ∀ (n: Node) (i: nat),
+    ⊢ <<< ∀∀ h mark next k, node n h mark next k >>>
+          getHeight #n @⊤
+      <<< node n h mark next k, RET #h >>>.
+
+  Parameter changeNext_spec : ∀ (n m m': Node) (i: nat),
+    ⊢  <<< ∀∀ h mark next k, node n h mark next k ∗ ⌜i < h⌝ >>>
+            changeNext #n #m #m' #i @⊤
+      <<< ∃∃ (success: bool) next',
+              node n h mark next' k
+            ∗ (match success with true => ⌜next !! i = Some m 
+                                            ∧ mark !!! i = false
+                                            ∧ next' = <[i := m']> next⌝
+                                | false => ⌜(next !! i ≠ Some m ∨ 
+                                              mark !!! i = true)
+                                            ∧ next' = next⌝ end),
+              RET (match success with true => SOMEV #() 
+                                    | false => NONEV end)  >>>.
+
+  Lemma maintenanceOp_insert_rec_spec N γ_t γ_s γ_m γ_td1 γ_td2 γ_ght k (n: Node) 
+    preds succs (ps ss: list Node) perm vs xs (h i: nat):
+    main_inv N γ_t γ_s γ_m γ_td1 γ_td2 γ_ght -∗
+      {{{   preds ↦∗ ((λ n0 : loc, #n0) <$> ps)
+          ∗ succs ↦∗ ((λ n0 : loc, #n0) <$> ss)
+          ∗ perm ↦∗ vs
+          ∗ ⌜vs = (fun n => # (LitInt (Z.of_nat n))) <$> xs⌝
+          ∗ ⌜xs ≡ₚ seq 1 (h-1)⌝ }}}
+         maintenanceOp_insert_rec #i #k #h #perm #preds #succs #n
+      {{{ (ps' ss': list Node),
+          RET #();
+            preds ↦∗ ((λ n0 : loc, #n0) <$> ps')
+          ∗ succs ↦∗ ((λ n0 : loc, #n0) <$> ss')
+          ∗ perm ↦∗ vs }}}.
+  Proof.
+    iIntros "#HInv". iIntros (Φ) "!# Hpre Hpost".
+    iDestruct "Hpre" as "(Hpreds & Hsuccs & Hperm & %Def_vs & %Perm_xs)".
+    wp_lam. wp_pures. 
+    destruct (bool_decide (Z.lt i (h - 1)%Z)) eqn: Hbool; wp_pures.
+    - rewrite bool_decide_eq_true in Hbool.
+      assert (is_Some (xs !! i)) as [idx Hidx].
+      { assert (i < length xs) as H'. rewrite Perm_xs seq_length. lia.
+        by rewrite lookup_lt_is_Some. }
+      wp_apply (wp_load_offset _ _ _ (DfracOwn 1) (i) (vs) #idx
+        with "[Hperm]"); try done.
+      { rewrite Def_vs. rewrite list_lookup_fmap. rewrite Hidx.
+        by simpl. }
+      iIntros "Hperm". wp_pures.
+      assert (is_Some (ps !! idx)) as [p Hp].
+      { admit. }
+      wp_apply (wp_load_offset _ _ _ (DfracOwn 1) (idx) _ #p
+        with "[Hpreds]"); try done.
+      { by rewrite list_lookup_fmap Hp /=. }
+      iIntros "Hpreds". wp_pures.
+      assert (is_Some (ss !! idx)) as [c Hc].
+      { admit. }
+      wp_apply (wp_load_offset _ _ _ (DfracOwn 1) (idx) _ #c
+        with "[Hsuccs]"); try done.
+      { by rewrite list_lookup_fmap Hc /=. }
+      iIntros "Hsuccs". wp_pures.
+      awp_apply changeNext_spec; try done.
+      iInv "HInv" as (M0 T0 s0) "(>Ds & >%Habs0 & >Hist & Help & >Templ)".
+      { admit. }
+      iDestruct "Templ" as "(SShot0 & Res & %PT0 & %Trans_M0)".
+      iDestruct "Res" as "(GKS & Nodes & Nodes_KS)".
+      iAssert (⌜p ∈ FP s0⌝)%I as %FP_p0.
+      { (* interpolation *) admit. }
+      rewrite (big_sepS_delete _ (FP s0) p); last by eauto.
+      iDestruct "Nodes" as "(Node_p & Nodes_rest)".
+      iAssert ((node p (Height s0 p) (Mark s0 p) (Next s0 p) (Key s0 p)) 
+        ∗ ⌜idx < Height s0 p⌝)%I with "[Node_p]" as "Hpre".
+      { admit. }
+      iAaccIntro with "Hpre".
+      { iIntros "(Node_p & _)". iModIntro. iFrame "Hpost Hperm Hpreds Hsuccs".
+        iNext; iExists M0, T0, s0. iFrame "∗%#". 
+        rewrite (big_sepS_delete _ (FP s0) p); last by eauto. iFrame. }
+      iIntros (success next')"(Node_p & Hif)".
+      destruct success; last first.
+      + iDestruct "Hif" as %[H' ->]. 
+        iModIntro. iSplitR "Hpost Hperm Hpreds Hsuccs".
+        { iNext. iExists M0, T0, s0. iFrame "∗%".
+          rewrite (big_sepS_delete _ (FP s0) p); last by eauto. iFrame. }
+        wp_pures. admit.
+      + admit.
+  Admitted.
+
+  Lemma maintenanceOp_insert_spec N γ_t γ_s γ_m γ_td1 γ_td2 γ_ght k (n:Node) preds succs 
+    ps ss:
+      main_inv N γ_t γ_s γ_m γ_td1 γ_td2 γ_ght -∗
+        {{{   preds ↦∗ ((λ n0 : loc, #n0) <$> ps)
+            ∗ succs ↦∗ ((λ n0 : loc, #n0) <$> ss) }}}
+           maintenanceOp_insert #k #preds #succs #n
+        {{{ (ps' ss': list Node),
+            RET #();
+              preds ↦∗ ((λ n0 : loc, #n0) <$> ps')
+            ∗ succs ↦∗ ((λ n0 : loc, #n0) <$> ss') }}}.
+  Proof.
+    iIntros "#HInv". iIntros (Φ) "!# (Hpreds & Hsuccs) Hpost".
+    wp_lam. wp_pures. awp_apply getHeight_spec; try done.
+    { admit. }
+    iInv "HInv" as (M0 T0 s0) "(>Ds & >%Habs0 & >Hist & Help & >Templ)".
+    { admit. }
+    iDestruct "Templ" as "(SShot0 & Res & %PT0 & %Trans_M0)".
+    iDestruct "Res" as "(GKS & Nodes & Nodes_KS)".
+    iAssert (⌜n ∈ FP s0⌝)%I as %FP_n0.
+    { (* interpolation *) admit. }
+    rewrite (big_sepS_delete _ (FP s0) n); last by eauto.
+    iDestruct "Nodes" as "(Node_n & Nodes_rest)".
+    iAaccIntro with "Node_n".
+    { iIntros "Node_n". iModIntro. iFrame.
+      iNext; iExists M0, T0, s0. iFrame "∗%#". 
+      rewrite (big_sepS_delete _ (FP s0) n); try done. iFrame. }
+    iIntros "Node_n". iSplitR "Hpreds Hsuccs Hpost".
+    { iModIntro. iNext; iExists M0, T0, s0. iFrame "∗%#". 
+      rewrite (big_sepS_delete _ (FP s0) n); try done. iFrame. }  
+    iModIntro. wp_pures. set h := Height s0 n. 
+    wp_apply permute_levels_spec; try done.
+    iIntros (perm vs xs)"(Hperm & %Def_vs & %Perm_xs)". wp_pures. 
+    wp_apply (maintenanceOp_insert_rec_spec with "[] [$Hperm $Hpreds $Hsuccs]"); 
+      try done.
+    iIntros (ps' ss')"(Hpreds & Hsuccs & Hperm)". 
+    iApply "Hpost". iFrame.
+  Admitted.
+
+End MAINTENANCEOP_INSERT.
+
